src/DenotationalSem.v
@@ -1,4 +1,5 @@
 Require Import List.
+Require Import Coq.Lists.ListSet.
 Import ListNotations.
 Require Import Stream.
 Require Import Unify.
@@ -41,6 +42,65 @@ Proof.
     subst. auto. }
 Qed.
 
+Lemma apply_gt_fun_fv
+      (f1 f2 : gt_fun)
+      (t : term)
+      (f_fv_eq : forall x, (In x (fv_term t)) -> gt_eq (f1 x) (f2 x)) :
+      gt_eq (apply_gt_fun f1 t) (apply_gt_fun f2 t).
+Proof.
+  induction t.
+  { simpl. apply f_fv_eq. simpl. auto. }
+  { unfold gt_eq. auto. }
+  { unfold gt_eq. simpl.
+    remember (apply_gt_fun f1 t1) as p11. destruct p11.
+    remember (apply_gt_fun f1 t2) as p12. destruct p12.
+    remember (apply_gt_fun f2 t1) as p21. destruct p21.
+    remember (apply_gt_fun f2 t2) as p22. destruct p22.
+    simpl.
+    assert (x = x1).
+    { apply IHt1. intros. apply f_fv_eq. unfold fv_term.
+      apply (set_union_intro name_eq_dec). left. auto. }
+    assert (x0 = x2).
+    { apply IHt2. intros. apply f_fv_eq. unfold fv_term.
+      apply (set_union_intro name_eq_dec). right. auto. }
+    subst. auto. }
+Qed.
+
+Lemma gt_fun_eq_trans
+      (f1 f2 f3 : gt_fun)
+      (eq12 : gt_fun_eq f1 f2)
+      (eq23 : gt_fun_eq f2 f3) :
+      gt_fun_eq f1 f3.
+Proof.
+  revert eq12 eq23. unfold gt_fun_eq. unfold gt_eq. intros.
+  rewrite eq12. auto.
+Qed.
+
+Lemma subst_of_gt
+      (t : term)
+      (s : subst)
+      (f : gt_fun)
+      (H : forall x : name, In x (fv_term t) -> image s x = Some (proj1_sig (f x))) :
+      apply_subst s t = proj1_sig (apply_gt_fun f t).
+Proof.
+  induction t.
+  { simpl. replace (image s n) with (Some (proj1_sig (f n))).
+    { auto. }
+    { symmetry. apply H. constructor. auto. } }
+  { auto. }
+  { simpl.
+    destruct (apply_gt_fun f t1).
+    destruct (apply_gt_fun f t2).
+    simpl.
+    replace x with (apply_subst s t1).
+    { replace x0 with (apply_subst s t2).
+      { auto. }
+      { apply IHt2. intros. apply H.
+        apply set_union_intro2. auto. } }
+    { apply IHt1. intros. apply H.
+      apply set_union_intro1. auto. } }
+Qed.
+
 Definition subst_gt_fun_compose (s : subst) (f : gt_fun) : gt_fun :=
   fun x => apply_gt_fun f (apply_subst s (Var x)).
 
@@ -59,6 +119,52 @@ Proof.
     red in IHt1. simpl in IHt1.
     red in IHt2. simpl in IHt2.
     subst. auto. }
+Qed.
+
+Lemma gt_fun_eq_compose
+      (f1 f2 : gt_fun)
+      (eq : gt_fun_eq f1 f2)
+      (s : subst) :
+      gt_fun_eq (subst_gt_fun_compose s f1) (subst_gt_fun_compose s f2).
+Proof.
+  unfold gt_fun_eq. unfold gt_fun_eq in eq. unfold subst_gt_fun_compose.
+  intro. induction (apply_subst s (Var x)).
+  { simpl. auto. }
+  { reflexivity. }
+  { unfold gt_eq. simpl.
+    remember (apply_gt_fun f1 t1) as p11. destruct p11.
+    remember (apply_gt_fun f1 t2) as p12. destruct p12.
+    remember (apply_gt_fun f2 t1) as p21. destruct p21.
+    remember (apply_gt_fun f2 t2) as p22. destruct p22.
+    simpl.
+    unfold gt_eq in IHt1. simpl in IHt1. rewrite IHt1.
+    unfold gt_eq in IHt2. simpl in IHt2. rewrite IHt2.
+    auto. }
+Qed.
+
+Lemma gt_fun_compose_eq
+      (f : gt_fun)
+      (s1 s2 : subst)
+      (eq : forall t, apply_subst s1 t = apply_subst s2 t) :
+      gt_fun_eq (subst_gt_fun_compose s1 f) (subst_gt_fun_compose s2 f).
+Proof.
+  unfold gt_fun_eq. unfold subst_gt_fun_compose. unfold gt_eq.
+  intro. rewrite eq. auto.
+Qed.
+
+Lemma subst_gt_fun_compose_assoc_subst
+      (f : gt_fun)
+      (s s' : subst) :
+      gt_fun_eq (subst_gt_fun_compose (compose s s') f)
+                (subst_gt_fun_compose s (subst_gt_fun_compose s' f)).
+Proof.
+  unfold gt_fun_eq. intros. unfold gt_eq.
+  replace (subst_gt_fun_compose (compose s s') f x) with
+          (apply_gt_fun (subst_gt_fun_compose (compose s s') f) (Var x)); auto.
+  rewrite gt_fun_apply_compose. rewrite compose_correctness.
+  replace (subst_gt_fun_compose s (subst_gt_fun_compose s' f) x) with
+          (apply_gt_fun (subst_gt_fun_compose s (subst_gt_fun_compose s' f)) (Var x)); auto.
+  rewrite gt_fun_apply_compose. rewrite gt_fun_apply_compose. auto.
 Qed.
 
 Inductive in_denotational_sem_goal : goal -> gt_fun -> Prop :=
@@ -136,4 +242,200 @@ Proof.
     { eapply in_denotational_sem_lev_monotone; eauto. apply PeanoNat.Nat.le_max_r. } }
   { destruct IHHdsg. eauto. }
   { destruct IHHdsg. eauto. }
+Qed.
+
+Lemma den_sem_fv_only
+      (f f' : gt_fun)
+      (g : goal)
+      (l : nat)
+      (ff'_eq : forall x, is_fv_of_goal x g -> gt_eq (f x) (f' x))
+      (Hgoal : in_denotational_sem_lev_goal l g f) :
+      in_denotational_sem_lev_goal l g f'.
+Proof.
+  revert ff'_eq. revert f'. induction Hgoal; intros.
+  { constructor. assert (gt_eq (apply_gt_fun f t1) (apply_gt_fun f' t1)).
+    { apply apply_gt_fun_fv. auto. }
+    assert (gt_eq (apply_gt_fun f t2) (apply_gt_fun f' t2)).
+    { apply apply_gt_fun_fv. auto. }
+    revert UnH H H0. unfold gt_eq. intros. congruence. }
+  { constructor. apply IHHgoal. intros.
+    apply ff'_eq. auto. }
+  { apply dslgDisjR. apply IHHgoal. intros.
+    apply ff'_eq. auto. }
+  { constructor.
+    { apply IHHgoal1; intros; apply ff'_eq; auto. }
+    { apply IHHgoal2; intros; apply ff'_eq; auto. } }
+  { remember (fun x => if name_eq_dec x a
+                         then fn a
+                         else f' x) as fn'.
+    apply dslgFresh with fn' a; auto.
+    { apply IHHgoal. intros. rewrite Heqfn'.
+      destruct (name_eq_dec x a).
+      { unfold gt_eq. subst. auto. }
+      { specialize (Hease _ n). red. rewrite Hease.
+        apply ff'_eq. eauto. } }
+    { rewrite Heqfn'. intros.
+      destruct (name_eq_dec x a); try contradiction.
+      reflexivity. } }
+  { constructor. apply IHHgoal. intros.
+    apply ff'_eq. constructor.
+    remember (MiniKanrenSyntax.P r). destruct d as [rel [Hcl Hco]].
+    simpl in H. red in Hcl. red in Hcl. auto. }
+Qed.
+
+
+Lemma den_sem_rename_var
+      (g1 g2 : goal)
+      (cg_g : consistent_goal g1)
+      (n : nat)
+      (g1Bound : forall x : name, is_fv_of_goal x g1 -> x < n)
+      (g2Bound : forall x : name, is_fv_of_goal x g2 -> x < n)
+      (a1 a2 : name)
+      (a12_neq : a1 <> a2)
+      (a2_fresh : ~ is_fv_of_goal a2 g1)
+      (sar : semiadequate_renaming a1 a2 g1 g2)
+      (fa1 fa2 : gt_fun)
+      (l : nat)
+      (Hgoal_f1 : in_denotational_sem_lev_goal l g1 fa1)
+      (f_switch : gt_eq (fa1 a1) (fa2 a2))
+      (f12_eq : forall x, x <> a1 -> x <> a2 -> gt_eq (fa1 x) (fa2 x)) :
+      in_denotational_sem_lev_goal l g2 fa2.
+Proof.
+  revert cg_g g1Bound g2Bound a12_neq a2_fresh sar Hgoal_f1 f_switch f12_eq.
+  revert g1 g2 n a1 a2 fa1 fa2.
+  induction l.
+  { intros. apply in_denotational_sem_zero_lev in Hgoal_f1. contradiction. }
+  { induction g1; intros; good_inversion Hgoal_f1; good_inversion sar; good_inversion cg_g.
+    { constructor.
+      etransitivity.
+      2: etransitivity.
+      2: apply UnH.
+      1-2: etransitivity.
+      1, 3: symmetry.
+      1, 4: apply gt_fun_apply_compose.
+      all: apply apply_gt_fun_fv; intros; unfold subst_gt_fun_compose;
+        simpl; destruct (Nat.eq_dec a1 x); subst; symmetry; auto;
+        apply f12_eq; auto; intro; subst; auto. }
+    { apply dslgDisjL; eauto. eapply IHg1_1; eauto. }
+    { apply dslgDisjR; eauto. eapply IHg1_2; eauto. }
+    { constructor; eauto.
+      { eapply IHg1_1; eauto. }
+      { eapply IHg1_2; eauto. } }
+    { apply den_sem_fv_only with fa1.
+      { intros; apply f12_eq; intro; subst; auto. }
+      { econstructor.
+        2: eauto.
+        all: eauto. } }
+    { rename g into fg. rename fn into fn1. rename a into a0. red in HBinding.
+      assert (very_fresh_var : exists y, a0 <> y /\ a2 <> y /\
+                                         (~ is_fv_of_goal y (Fresh fg)) /\
+                                         (~ is_fv_of_goal y (Fresh rfg))).
+      { destruct (name_eq_dec a0 n); destruct (name_eq_dec a0 (S n));
+        destruct (name_eq_dec a2 n); destruct (name_eq_dec a2 (S n)); subst; try omega.
+        5, 6, 8, 9: exists n.
+        1, 3, 9: exists (S n).
+        4, 5: exists (S (S n)).
+        all: repeat split; try omega.
+        all: intro CH; try apply g1Bound in CH; try apply g2Bound in CH; omega. }
+      destruct very_fresh_var as [a3 [a03_neq [a23_neq [a3_fresh a3_rfresh]]]].
+      assert (a13_neq : a1 <> a3).
+      { intro; subst; auto. }
+      remember (fun x => if name_eq_dec x a3
+                           then fn1 a0
+                           else if name_eq_dec x a0
+                                  then fa2 a0
+                                  else fn1 x) as fn0 eqn:fn0_def.
+      assert (AH0 : in_denotational_sem_lev_goal (S l) (fg a3) fn0).
+      { subst.
+        apply H with a0 (max n (max (S a0) (S a3))) a0 a3 fn1; eauto.
+        { intros. destruct (name_eq_dec x a0); subst.
+          { zify. omega. }
+          { assert (x < n); eauto. zify. omega. } }
+        { intros. destruct (name_eq_dec x a3); subst.
+          { zify. omega. }
+          { assert (x < n); eauto. zify. omega. } }
+        { destruct (name_eq_dec a3 a3); subst.
+          { reflexivity. }
+          { contradiction. } }
+        { intros. destruct (name_eq_dec x a3).
+          { contradiction. }
+          { destruct (name_eq_dec x a0).
+            { contradiction. }
+            { reflexivity. } } } }
+      remember (fun x => if name_eq_dec x a2
+                           then fn0 a1
+                           else if name_eq_dec x a1
+                                  then fa2 a1
+                                  else fn0 x) as fn2 eqn:fn2_def.
+      assert (AH2 : in_denotational_sem_lev_goal (S l) (rfg a3) fn2).
+      { apply H with a3 (max n (max (S a0) (S a3))) a1 a2 fn0; subst; eauto.
+        { intros. destruct (name_eq_dec x a3); subst.
+          { zify. omega. }
+          { assert (x < n); eauto. zify. omega. } }
+        { intros. destruct (name_eq_dec x a3); subst.
+          { zify. omega. }
+          { assert (x < n); eauto. zify. omega. } }
+        { simpl. destruct (name_eq_dec a2 a2); subst.
+          { reflexivity. }
+          { contradiction. } }
+        { intros. simpl. destruct (name_eq_dec x a2).
+          { contradiction. }
+          { destruct (name_eq_dec x a1).
+            { contradiction. }
+            { reflexivity. } } } }
+      econstructor; eauto.
+      intros. subst. destruct (name_eq_dec x a2); subst.
+      { destruct (name_eq_dec a1 a0); subst.
+        { contradiction. }
+        { destruct (name_eq_dec a1 a3); subst.
+          { contradiction. }
+          { etransitivity.
+            { apply Hease. auto. }
+            { auto. } } } }
+      { destruct (name_eq_dec x a1); subst.
+        { reflexivity. }
+        { destruct (name_eq_dec x a3).
+          { contradiction. }
+          { destruct (name_eq_dec x a0); subst.
+            { reflexivity. }
+            { etransitivity.
+              { apply Hease. auto. }
+              { apply f12_eq; auto. } } } } } }
+    { rename n into r. rename n0 into n.
+      remember (MiniKanrenSyntax.P r) as d. destruct d as [rel [Hcl Hco]].
+      red in Hco. destruct (Hco t) as [Hcog Hcof].
+      red in Hcl. unfold closed_goal_in_context in Hcl.
+      econstructor.
+      rewrite <- Heqd. simpl.
+      eapply IHl.
+      7: eauto.
+      all: simpl; eauto. } }
+Qed.
+
+Lemma den_sem_another_fresh_var
+      (b : name -> goal)
+      (cg : consistent_goal (Fresh b))
+      (n : nat)
+      (freshBound : forall x : name, is_fv_of_goal x (Fresh b) -> x < n)
+      (a1 a2 : name)
+      (a1_fresh : ~ is_fv_of_goal a1 (Fresh b))
+      (a2_fresh : ~ is_fv_of_goal a2 (Fresh b))
+      (fa1 fa2 : gt_fun)
+      (l : nat)
+      (Hgoal_f1 : in_denotational_sem_lev_goal l (b a1) fa1)
+      (f_switch : gt_eq (fa1 a1) (fa2 a2))
+      (f12_eq : forall x, x <> a1 -> x <> a2 -> gt_eq (fa1 x) (fa2 x)) :
+      in_denotational_sem_lev_goal l (b a2) fa2.
+Proof.
+  destruct (name_eq_dec a1 a2); subst.
+  { apply den_sem_fv_only with fa1; auto.
+    intros. destruct (name_eq_dec x a2); subst; auto. }
+  { good_inversion cg. red in HBinding.
+    eapply den_sem_rename_var with (g1 := (b a1)) (n := max n (max (S a1) (S a2))); eauto.
+    { intros. destruct (name_eq_dec x a1); subst.
+      { zify. omega. }
+      { assert (x < n); eauto. zify. omega. } }
+    { intros. destruct (name_eq_dec x a2); subst.
+      { zify. omega. }
+      { assert (x < n); eauto. zify. omega. } } }
 Qed.
