src/SemanticsEquivalence.v
@@ -11,6 +11,72 @@ Require Import Omega.
 Definition in_denotational_sem_subst (s : subst) (f : gt_fun) : Prop :=
   exists (f' : gt_fun), gt_fun_eq (subst_gt_fun_compose s f') f.
 
+Lemma set_empty_union
+      (s1 s2 : var_set)
+      (eq : var_set_union s1 s2 = var_set_empty) :
+      s1 = var_set_empty /\ s2 = var_set_empty.
+Proof.
+  split.
+  { destruct s1; auto.
+    assert (In n var_set_empty).
+    { rewrite <- eq. apply set_union_intro. left. constructor. auto. }
+    inversion H. }
+  { destruct s2; auto.
+    assert (In n var_set_empty).
+    { rewrite <- eq. apply set_union_intro. right. constructor. auto. }
+    inversion H. }
+Qed.
+
+Lemma unfier_from_gt_unifier
+      (t1 t2 : term)
+      (f : gt_fun)
+      (f_unifies : gt_eq (apply_gt_fun f t1) (apply_gt_fun f t2)) :
+      exists s, unifier s t1 t2 /\ in_denotational_sem_subst s f.
+Proof.
+  remember (map (fun x => (x, proj1_sig (f x))) (var_set_union (fv_term t1) (fv_term t2))) as s.
+  exists s. split.
+  { red. red in f_unifies.
+    assert (apply_subst s t1 = proj1_sig (apply_gt_fun f t1)).
+    { clear f_unifies.
+      assert (forall x, In x (fv_term t1) -> image s x = Some (proj1_sig (f x))).
+      { intros. assert (In x (var_set_union (fv_term t1) (fv_term t2))).
+        { apply set_union_intro1. auto. }
+        remember (var_set_union (fv_term t1) (fv_term t2)).
+        subst. apply map_image. auto. }
+      apply subst_of_gt. auto. }
+    assert (apply_subst s t2 = proj1_sig (apply_gt_fun f t2)).
+    { clear f_unifies.
+      assert (forall x, In x (fv_term t2) -> image s x = Some (proj1_sig (f x))).
+      { intros. assert (In x (var_set_union (fv_term t1) (fv_term t2))).
+        { apply set_union_intro2. auto. }
+        remember (var_set_union (fv_term t1) (fv_term t2)).
+        subst. apply map_image. auto. }
+      apply subst_of_gt. auto. }
+    congruence. }
+  { red. exists f. red. intros x. unfold subst_gt_fun_compose.
+    unfold apply_subst. destruct (image s x) eqn:eq.
+    { destruct (f x) eqn:eqfx.
+      assert (x0 = t).
+      { unfold image in eq.
+        remember (var_set_union (fv_term t1) (fv_term t2)). clear Heqv.
+        revert Heqs. revert v.
+        induction s.
+        { inversion eq. }
+        { intros. destruct a as [y t0]. destruct v; good_inversion Heqs.
+          destruct (Nat.eq_dec n x).
+          { good_inversion eq. rewrite eqfx. auto. }
+          { apply IHs with v; auto. } } }
+      subst. red. simpl. clear eqfx. clear eq. induction t.
+      { inversion e. }
+      { auto. }
+      { simpl in e. apply set_empty_union in e. destruct e.
+        apply IHt1 in H. apply IHt2 in H0. simpl.
+        destruct (apply_gt_fun f t3). simpl in H.
+        destruct (apply_gt_fun f t4). simpl in H0.
+        simpl. subst. auto. } }
+    { red. auto. } }
+Qed.
+
 Inductive in_denotational_sem_state' : state' -> gt_fun -> Prop :=
 | dsst'Leaf : forall g s n f (Hgoal : in_denotational_sem_goal g f)
                              (Hsubst : in_denotational_sem_subst s f),
@@ -83,7 +149,7 @@ Proof.
   { good_inversion Hst'. good_inversion Hst'0. auto. }
   { good_inversion wfState. good_inversion Hst'.
     constructor; auto. econstructor; eauto.
-    intros HIn. apply freshCorrect in HIn.
+    intros HIn. apply FVLTCounter in HIn.
     { omega. }
     { reflexivity. } }
   { good_inversion Hst'. auto. }
@@ -147,479 +213,10 @@ Proof.
   assert (in_denotational_sem_state st f).
   { eapply search_correctness_generalized; eauto.
     subst. constructor. constructor.
-    intros. apply HC in H. apply first_nats_less. auto. }
+    { intros. good_inversion H. good_inversion H0. }
+    { intros. good_inversion H. destruct H0 as [t1 [H1 _]]. good_inversion H1. }
+    { intros. apply HC in H. apply first_nats_less. auto. } }
   subst. inversion H. inversion Hst'. auto.
-Qed.
-
-Lemma set_empty_union
-      (s1 s2 : var_set)
-      (eq : var_set_union s1 s2 = var_set_empty) :
-      s1 = var_set_empty /\ s2 = var_set_empty.
-Proof.
-  split.
-  { destruct s1; auto.
-    assert (In n var_set_empty).
-    { rewrite <- eq. apply set_union_intro. left. constructor. auto. }
-    inversion H. }
-  { destruct s2; auto.
-    assert (In n var_set_empty).
-    { rewrite <- eq. apply set_union_intro. right. constructor. auto. }
-    inversion H. }
-Qed.
-
-Lemma map_image
-      (f : name -> term)
-      (v : var_set)
-      (x : name)
-      (HIn : In x v) :
-      image (map (fun x0 : name => (x0, f x0)) v) x = Some (f x).
-Proof.
-  induction v.
-  { contradiction. }
-  { simpl. destruct (Nat.eq_dec a x).
-    { subst. auto. }
-    { apply IHv. destruct HIn; auto. contradiction. } }
-Qed.
-
-Lemma subst_of_gt
-      (t : term)
-      (s : subst)
-      (f : gt_fun)
-      (H : forall x : name, In x (fv_term t) -> image s x = Some (proj1_sig (f x))) :
-      apply_subst s t = proj1_sig (apply_gt_fun f t).
-Proof.
-  induction t.
-  { simpl. replace (image s n) with (Some (proj1_sig (f n))).
-    { auto. }
-    { symmetry. apply H. constructor. auto. } }
-  { auto. }
-  { simpl.
-    destruct (apply_gt_fun f t1).
-    destruct (apply_gt_fun f t2).
-    simpl.
-    replace x with (apply_subst s t1).
-    { replace x0 with (apply_subst s t2).
-      { auto. }
-      { apply IHt2. intros. apply H.
-        apply set_union_intro2. auto. } }
-    { apply IHt1. intros. apply H.
-      apply set_union_intro1. auto. } }
-Qed.
-
-Lemma unfier_from_gt_unifier
-      (t1 t2 : term)
-      (f : gt_fun)
-      (f_unifies : gt_eq (apply_gt_fun f t1) (apply_gt_fun f t2)) :
-      exists s, unifier s t1 t2 /\ in_denotational_sem_subst s f.
-Proof.
-  remember (map (fun x => (x, proj1_sig (f x))) (var_set_union (fv_term t1) (fv_term t2))) as s.
-  exists s. split.
-  { red. red in f_unifies.
-    assert (apply_subst s t1 = proj1_sig (apply_gt_fun f t1)).
-    { clear f_unifies.
-      assert (forall x, In x (fv_term t1) -> image s x = Some (proj1_sig (f x))).
-      { intros. assert (In x (var_set_union (fv_term t1) (fv_term t2))).
-        { apply set_union_intro1. auto. }
-        remember (var_set_union (fv_term t1) (fv_term t2)).
-        subst. apply map_image. auto. }
-      apply subst_of_gt. auto. }
-    assert (apply_subst s t2 = proj1_sig (apply_gt_fun f t2)).
-    { clear f_unifies.
-      assert (forall x, In x (fv_term t2) -> image s x = Some (proj1_sig (f x))).
-      { intros. assert (In x (var_set_union (fv_term t1) (fv_term t2))).
-        { apply set_union_intro2. auto. }
-        remember (var_set_union (fv_term t1) (fv_term t2)).
-        subst. apply map_image. auto. }
-      apply subst_of_gt. auto. }
-    congruence. }
-  { red. exists f. red. intros x. unfold subst_gt_fun_compose.
-    unfold apply_subst. destruct (image s x) eqn:eq.
-    { destruct (f x) eqn:eqfx.
-      assert (x0 = t).
-      { unfold image in eq.
-        remember (var_set_union (fv_term t1) (fv_term t2)). clear Heqv.
-        revert Heqs. revert v.
-        induction s.
-        { inversion eq. }
-        { intros. destruct a as [y t0]. destruct v; good_inversion Heqs.
-          destruct (Nat.eq_dec n x).
-          { good_inversion eq. rewrite eqfx. auto. }
-          { apply IHs with v; auto. } } }
-      subst. red. simpl. clear eqfx. clear eq. induction t.
-      { inversion e. }
-      { auto. }
-      { simpl in e. apply set_empty_union in e. destruct e.
-        apply IHt1 in H. apply IHt2 in H0. simpl.
-        destruct (apply_gt_fun f t3). simpl in H.
-        destruct (apply_gt_fun f t4). simpl in H0.
-        simpl. subst. auto. } }
-    { red. auto. } }
-Qed.
-
-Lemma gt_fun_eq_trans
-      (f1 f2 f3 : gt_fun)
-      (eq12 : gt_fun_eq f1 f2)
-      (eq23 : gt_fun_eq f2 f3) :
-      gt_fun_eq f1 f3.
-Proof.
-  revert eq12 eq23. unfold gt_fun_eq. unfold gt_eq. intros.
-  rewrite eq12. auto.
-Qed.
-
-Lemma gt_fun_eq_compose
-      (f1 f2 : gt_fun)
-      (eq : gt_fun_eq f1 f2)
-      (s : subst) :
-      gt_fun_eq (subst_gt_fun_compose s f1) (subst_gt_fun_compose s f2).
-Proof.
-  unfold gt_fun_eq. unfold gt_fun_eq in eq. unfold subst_gt_fun_compose.
-  intro. induction (apply_subst s (Var x)).
-  { simpl. auto. }
-  { reflexivity. }
-  { unfold gt_eq. simpl.
-    remember (apply_gt_fun f1 t1) as p11. destruct p11.
-    remember (apply_gt_fun f1 t2) as p12. destruct p12.
-    remember (apply_gt_fun f2 t1) as p21. destruct p21.
-    remember (apply_gt_fun f2 t2) as p22. destruct p22.
-    simpl.
-    unfold gt_eq in IHt1. simpl in IHt1. rewrite IHt1.
-    unfold gt_eq in IHt2. simpl in IHt2. rewrite IHt2.
-    auto. }
-Qed.
-
-Lemma gt_fun_compose_eq
-      (f : gt_fun)
-      (s1 s2 : subst)
-      (eq : forall t, apply_subst s1 t = apply_subst s2 t) :
-      gt_fun_eq (subst_gt_fun_compose s1 f) (subst_gt_fun_compose s2 f).
-Proof.
-  unfold gt_fun_eq. unfold subst_gt_fun_compose. unfold gt_eq.
-  intro. rewrite eq. auto.
-Qed.
-
-Lemma subst_gt_fun_compose_assoc_subst
-      (f : gt_fun)
-      (s s' : subst) :
-      gt_fun_eq (subst_gt_fun_compose (compose s s') f)
-                (subst_gt_fun_compose s (subst_gt_fun_compose s' f)).
-Proof.
-  unfold gt_fun_eq. intros. unfold gt_eq.
-  replace (subst_gt_fun_compose (compose s s') f x) with
-          (apply_gt_fun (subst_gt_fun_compose (compose s s') f) (Var x)); auto.
-  rewrite gt_fun_apply_compose. rewrite compose_correctness.
-  replace (subst_gt_fun_compose s (subst_gt_fun_compose s' f) x) with
-          (apply_gt_fun (subst_gt_fun_compose s (subst_gt_fun_compose s' f)) (Var x)); auto.
-  rewrite gt_fun_apply_compose. rewrite gt_fun_apply_compose. auto.
-Qed.
-
-Lemma counter_in_answer
-      (g : goal)
-      (s sr : subst)
-      (n nr : nat)
-      (tr : trace)
-      (OP : op_sem (State (Leaf g s n)) tr)
-      (HIn : in_stream (Answer sr nr) tr) :
-      n <= nr.
-Proof.
-  remember (Leaf g s n) as st'.
-  assert (forall n', is_counter_of_state' n' st' -> n <= n').
-  { intros. subst. good_inversion H. auto. }
-  clear Heqst'. revert H OP. revert n st'.
-  remember (Answer sr nr). induction HIn; intros; subst.
-  { good_inversion OP. apply counter_in_answer in EV. auto. }
-  { good_inversion OP. destruct st.
-    { good_inversion OP0. good_inversion HIn. }
-    { apply IHHIn with s0; auto. intros.
-      specialize (counter_in_next_state _ _ _ _ EV H0). intros.
-      destruct H1. destruct H1. apply H in H2.
-      eapply le_trans; eauto. } }
-Qed.
-
-Lemma prod_op_sem_in
-      (st' : state')
-      (g : goal)
-      (s : subst)
-      (n : nat)
-      (t1 t2 t : trace)
-      (r : label)
-      (OP : op_sem (State (Prod st' g)) t)
-      (OP1 : op_sem (State st') t1)
-      (OP2 : op_sem (State (Leaf g s n)) t2)
-      (HIn1 : in_stream (Answer s n) t1)
-      (HIn2 : in_stream r t2) :
-      in_stream r t.
-Proof.
-  revert OP OP1. revert t st'. remember (Answer s n) as r1.
-  induction HIn1; intros; subst.
-  { good_inversion OP1. good_inversion OP.
-    good_inversion EV0; specialize (eval_step_unique _ _ _ _ _ EV H3);
-    intro eqs; destruct eqs; subst; good_inversion H.
-    { constructor. specialize (op_sem_unique _ _ _ OP2 OP1).
-      intros. eapply in_equal_streams; eauto. }
-    { constructor. specialize (op_sem_exists (State (Leaf g s0 n0))).
-      intro H. destruct H as [t3 OP3].
-      specialize (op_sem_exists (State (Prod st'0 g))).
-      intro H. destruct H as [t4 OP4].
-      specialize (sum_op_sem _ _ _ _ _ OP3 OP4 OP1).
-      intro interH. eapply interleave_in in interH.
-      eapply interH. left. specialize (op_sem_unique _ _ _ OP2 OP3).
-      intros. eapply in_equal_streams; eauto. } }
-  { specialize (IHHIn1 eq_refl).
-    good_inversion OP1. good_inversion OP.
-    good_inversion EV0; specialize (eval_step_unique _ _ _ _ _ EV H3);
-    intro eqs; destruct eqs; subst.
-    1-2: good_inversion OP0; good_inversion HIn1.
-    { constructor. eapply IHHIn1; eauto. }
-    { constructor. specialize (op_sem_exists (State (Leaf g s0 n0))).
-      intro H. destruct H as [t3 OP3].
-      specialize (op_sem_exists (State (Prod st'0 g))).
-      intro H. destruct H as [t4 OP4].
-      specialize (sum_op_sem _ _ _ _ _ OP3 OP4 OP1).
-      intro interH. eapply interleave_in in interH.
-      eapply interH. right. eapply IHHIn1; eauto. } }
-Qed.
-
-Lemma apply_gt_fun_fv
-      (f1 f2 : gt_fun)
-      (t : term)
-      (f_fv_eq : forall x, (In x (fv_term t)) -> gt_eq (f1 x) (f2 x)) :
-      gt_eq (apply_gt_fun f1 t) (apply_gt_fun f2 t).
-Proof.
-  induction t.
-  { simpl. apply f_fv_eq. simpl. auto. }
-  { unfold gt_eq. auto. }
-  { unfold gt_eq. simpl.
-    remember (apply_gt_fun f1 t1) as p11. destruct p11.
-    remember (apply_gt_fun f1 t2) as p12. destruct p12.
-    remember (apply_gt_fun f2 t1) as p21. destruct p21.
-    remember (apply_gt_fun f2 t2) as p22. destruct p22.
-    simpl.
-    assert (x = x1).
-    { apply IHt1. intros. apply f_fv_eq. unfold fv_term.
-      apply (set_union_intro name_eq_dec). left. auto. }
-    assert (x0 = x2).
-    { apply IHt2. intros. apply f_fv_eq. unfold fv_term.
-      apply (set_union_intro name_eq_dec). right. auto. }
-    subst. auto. }
-Qed.
-
-Lemma well_formed_subst_in_state_dom
-      (g : goal)
-      (s : subst)
-      (n : nat)
-      (wfSt' : well_formed_state' (Leaf g s n))
-      (x : name)
-      (n_le_x : n <= x) :
-      image s x = None.
-Proof. admit. Admitted.
-
-Lemma well_formed_subst_in_state_vran
-      (g : goal)
-      (s : subst)
-      (n : nat)
-      (wfSt' : well_formed_state' (Leaf g s n))
-      (x : name)
-      (t : term)
-      (img_x : image s x = Some t)
-      (v : name)
-      (v_in : In v (fv_term t)) :
-      v < n.
-Proof. admit. Admitted.
-
-Lemma den_sem_fv_only
-      (f f' : gt_fun)
-      (g : goal)
-      (l : nat)
-      (ff'_eq : forall x, is_fv_of_goal x g -> gt_eq (f x) (f' x))
-      (Hgoal : in_denotational_sem_lev_goal l g f) :
-      in_denotational_sem_lev_goal l g f'.
-Proof.
-  revert ff'_eq. revert f'. induction Hgoal; intros.
-  { constructor. assert (gt_eq (apply_gt_fun f t1) (apply_gt_fun f' t1)).
-    { apply apply_gt_fun_fv. auto. }
-    assert (gt_eq (apply_gt_fun f t2) (apply_gt_fun f' t2)).
-    { apply apply_gt_fun_fv. auto. }
-    revert UnH H H0. unfold gt_eq. intros. congruence. }
-  { constructor. apply IHHgoal. intros.
-    apply ff'_eq. auto. }
-  { apply dslgDisjR. apply IHHgoal. intros.
-    apply ff'_eq. auto. }
-  { constructor.
-    { apply IHHgoal1; intros; apply ff'_eq; auto. }
-    { apply IHHgoal2; intros; apply ff'_eq; auto. } }
-  { remember (fun x => if name_eq_dec x a
-                         then fn a
-                         else f' x) as fn'.
-    apply dslgFresh with fn' a; auto.
-    { apply IHHgoal. intros. rewrite Heqfn'.
-      destruct (name_eq_dec x a).
-      { unfold gt_eq. subst. auto. }
-      { specialize (Hease _ n). red. rewrite Hease.
-        apply ff'_eq. eauto. } }
-    { rewrite Heqfn'. intros.
-      destruct (name_eq_dec x a); try contradiction.
-      reflexivity. } }
-  { constructor. apply IHHgoal. intros.
-    apply ff'_eq. constructor.
-    remember (MiniKanrenSyntax.P r). destruct d as [rel [Hcl Hco]].
-    simpl in H. red in Hcl. red in Hcl. auto. }
-Qed.
-
-
-Lemma den_sem_rename_var
-      (g1 g2 : goal)
-      (cg_g : consistent_goal g1)
-      (n : nat)
-      (g1Bound : forall x : name, is_fv_of_goal x g1 -> x < n)
-      (g2Bound : forall x : name, is_fv_of_goal x g2 -> x < n)
-      (a1 a2 : name)
-      (a12_neq : a1 <> a2)
-      (a2_fresh : ~ is_fv_of_goal a2 g1)
-      (sar : semiadequate_renaming a1 a2 g1 g2)
-      (fa1 fa2 : gt_fun)
-      (l : nat)
-      (Hgoal_f1 : in_denotational_sem_lev_goal l g1 fa1)
-      (f_switch : gt_eq (fa1 a1) (fa2 a2))
-      (f12_eq : forall x, x <> a1 -> x <> a2 -> gt_eq (fa1 x) (fa2 x)) :
-      in_denotational_sem_lev_goal l g2 fa2.
-Proof.
-  revert cg_g g1Bound g2Bound a12_neq a2_fresh sar Hgoal_f1 f_switch f12_eq.
-  revert g1 g2 n a1 a2 fa1 fa2.
-  induction l.
-  { intros. apply in_denotational_sem_zero_lev in Hgoal_f1. contradiction. }
-  { induction g1; intros; good_inversion Hgoal_f1; good_inversion sar; good_inversion cg_g.
-    { constructor.
-      etransitivity.
-      2: etransitivity.
-      2: apply UnH.
-      1-2: etransitivity.
-      1, 3: symmetry.
-      1, 4: apply gt_fun_apply_compose.
-      all: apply apply_gt_fun_fv; intros; unfold subst_gt_fun_compose;
-        simpl; destruct (Nat.eq_dec a1 x); subst; symmetry; auto;
-        apply f12_eq; auto; intro; subst; auto. }
-    { apply dslgDisjL; eauto. eapply IHg1_1; eauto. }
-    { apply dslgDisjR; eauto. eapply IHg1_2; eauto. }
-    { constructor; eauto.
-      { eapply IHg1_1; eauto. }
-      { eapply IHg1_2; eauto. } }
-    { apply den_sem_fv_only with fa1.
-      { intros; apply f12_eq; intro; subst; auto. }
-      { econstructor.
-        2: eauto.
-        all: eauto. } }
-    { rename g into fg. rename fn into fn1. rename a into a0. red in HBinding.
-      assert (very_fresh_var : exists y, a0 <> y /\ a2 <> y /\
-                                         (~ is_fv_of_goal y (Fresh fg)) /\
-                                         (~ is_fv_of_goal y (Fresh rfg))).
-      { destruct (name_eq_dec a0 n); destruct (name_eq_dec a0 (S n));
-        destruct (name_eq_dec a2 n); destruct (name_eq_dec a2 (S n)); subst; try omega.
-        5, 6, 8, 9: exists n.
-        1, 3, 9: exists (S n).
-        4, 5: exists (S (S n)).
-        all: repeat split; try omega.
-        all: intro CH; try apply g1Bound in CH; try apply g2Bound in CH; omega. }
-      destruct very_fresh_var as [a3 [a03_neq [a23_neq [a3_fresh a3_rfresh]]]].
-      assert (a13_neq : a1 <> a3).
-      { intro; subst; auto. }
-      remember (fun x => if name_eq_dec x a3
-                           then fn1 a0
-                           else if name_eq_dec x a0
-                                  then fa2 a0
-                                  else fn1 x) as fn0 eqn:fn0_def.
-      assert (AH0 : in_denotational_sem_lev_goal (S l) (fg a3) fn0).
-      { subst.
-        apply H with a0 (max n (max (S a0) (S a3))) a0 a3 fn1; eauto.
-        { intros. destruct (name_eq_dec x a0); subst.
-          { zify. omega. }
-          { assert (x < n); eauto. zify. omega. } }
-        { intros. destruct (name_eq_dec x a3); subst.
-          { zify. omega. }
-          { assert (x < n); eauto. zify. omega. } }
-        { destruct (name_eq_dec a3 a3); subst.
-          { reflexivity. }
-          { contradiction. } }
-        { intros. destruct (name_eq_dec x a3).
-          { contradiction. }
-          { destruct (name_eq_dec x a0).
-            { contradiction. }
-            { reflexivity. } } } }
-      remember (fun x => if name_eq_dec x a2
-                           then fn0 a1
-                           else if name_eq_dec x a1
-                                  then fa2 a1
-                                  else fn0 x) as fn2 eqn:fn2_def.
-      assert (AH2 : in_denotational_sem_lev_goal (S l) (rfg a3) fn2).
-      { apply H with a3 (max n (max (S a0) (S a3))) a1 a2 fn0; subst; eauto.
-        { intros. destruct (name_eq_dec x a3); subst.
-          { zify. omega. }
-          { assert (x < n); eauto. zify. omega. } }
-        { intros. destruct (name_eq_dec x a3); subst.
-          { zify. omega. }
-          { assert (x < n); eauto. zify. omega. } }
-        { simpl. destruct (name_eq_dec a2 a2); subst.
-          { reflexivity. }
-          { contradiction. } }
-        { intros. simpl. destruct (name_eq_dec x a2).
-          { contradiction. }
-          { destruct (name_eq_dec x a1).
-            { contradiction. }
-            { reflexivity. } } } }
-      econstructor; eauto.
-      intros. subst. destruct (name_eq_dec x a2); subst.
-      { destruct (name_eq_dec a1 a0); subst.
-        { contradiction. }
-        { destruct (name_eq_dec a1 a3); subst.
-          { contradiction. }
-          { etransitivity.
-            { apply Hease. auto. }
-            { auto. } } } }
-      { destruct (name_eq_dec x a1); subst.
-        { reflexivity. }
-        { destruct (name_eq_dec x a3).
-          { contradiction. }
-          { destruct (name_eq_dec x a0); subst.
-            { reflexivity. }
-            { etransitivity.
-              { apply Hease. auto. }
-              { apply f12_eq; auto. } } } } } }
-    { rename n into r. rename n0 into n.
-      remember (MiniKanrenSyntax.P r) as d. destruct d as [rel [Hcl Hco]].
-      red in Hco. destruct (Hco t) as [Hcog Hcof].
-      red in Hcl. unfold closed_goal_in_context in Hcl.
-      econstructor.
-      rewrite <- Heqd. simpl.
-      eapply IHl.
-      7: eauto.
-      all: simpl; eauto. } }
-Qed.
-
-Lemma den_sem_another_fresh_var
-      (b : name -> goal)
-      (cg : consistent_goal (Fresh b))
-      (n : nat)
-      (freshBound : forall x : name, is_fv_of_goal x (Fresh b) -> x < n)
-      (a1 a2 : name)
-      (a1_fresh : ~ is_fv_of_goal a1 (Fresh b))
-      (a2_fresh : ~ is_fv_of_goal a2 (Fresh b))
-      (fa1 fa2 : gt_fun)
-      (l : nat)
-      (Hgoal_f1 : in_denotational_sem_lev_goal l (b a1) fa1)
-      (f_switch : gt_eq (fa1 a1) (fa2 a2))
-      (f12_eq : forall x, x <> a1 -> x <> a2 -> gt_eq (fa1 x) (fa2 x)) :
-      in_denotational_sem_lev_goal l (b a2) fa2.
-Proof.
-  destruct (name_eq_dec a1 a2); subst.
-  { apply den_sem_fv_only with fa1; auto.
-    intros. destruct (name_eq_dec x a2); subst; auto. }
-  { good_inversion cg. red in HBinding.
-    eapply den_sem_rename_var with (g1 := (b a1)) (n := max n (max (S a1) (S a2))); eauto.
-    { intros. destruct (name_eq_dec x a1); subst.
-      { zify. omega. }
-      { assert (x < n); eauto. zify. omega. } }
-    { intros. destruct (name_eq_dec x a2); subst.
-      { zify. omega. }
-      { assert (x < n); eauto. zify. omega. } } }
 Qed.
 
 Lemma search_completeness_generalized
@@ -683,14 +280,17 @@ Proof.
     { good_inversion Hgoal. good_inversion HOP. inversion EV; subst.
       specialize (op_sem_exists (State (Leaf g1 s n))). intro p1. destruct p1 as [t1 OP1].
       assert (wfst'1 : well_formed_state' (Leaf g1 s n)).
-      { constructor. good_inversion wfSt'. auto. }
+      { constructor; good_inversion wfSt'; auto. }
       specialize (IHg1 f s n Hcg1 Hg1 Hsubst wfst'1 t1 OP1).
       destruct IHg1 as [f' [HinDA ff'_eq]]. red in HinDA.
       destruct HinDA as [s' [n' [Hinstr' HDAS']]].
       specialize (op_sem_exists (State (Leaf g2 s' n'))). intro p2. destruct p2 as [t2 OP2].
-      specialize (counter_in_answer _ _ _ _ _ _ OP1 Hinstr'). intro n_le_n'.
+      specialize (counter_in_trace _ _ _ _ _ _ OP1 Hinstr'). intro n_le_n'.
       assert (wfst'2 : well_formed_state' (Leaf g2 s' n')).
-      { constructor. good_inversion wfSt'. intros.
+      { good_inversion wfSt'.
+        specialize (well_formed_subst_in_trace _ (wfNonEmpty _ wfst'1)  _ OP1 _ _ Hinstr').
+        intros. destruct H.
+        constructor; auto. intros.
         apply lt_le_trans with n; auto. }
       assert (Hg2' : in_denotational_sem_lev_goal (S l) g2 f').
       { apply den_sem_fv_only with f; auto. intros. apply ff'_eq.
@@ -719,13 +319,15 @@ Proof.
       assert (H_n_is_fresh : forall x, In n (fv_term (apply_subst s (Var x))) -> x = n).
       { intros. simpl in H0.
         destruct (image s x) eqn:eq.
-        { specialize (well_formed_subst_in_state_vran _ _ _ wfSt' _ _ eq _ H0).
+        { assert (n < n).
+          { good_inversion wfSt'. apply vranLTCounter.
+            red. eauto. }
           omega. }
         { simpl in H0. destruct H0; try contradiction. auto. } }
       assert (Hgn : in_denotational_sem_lev_goal (S l) (g n) fn).
       { rewrite Heqfn. good_inversion wfSt'.
         apply den_sem_another_fresh_var with n a fa; auto.
-        { intro C. apply freshCorrect in C. omega. }
+        { intro C. apply FVLTCounter in C. omega. }
         { destruct (name_eq_dec n n); try contradiction. reflexivity. }
         { intros. destruct (name_eq_dec x n); try contradiction.
           destruct (name_eq_dec x a); try contradiction. reflexivity. } }
@@ -733,8 +335,10 @@ Proof.
       { red. exists fs'. red. intros. red. unfold subst_gt_fun_compose.
         rewrite Heqfs'. rewrite Heqfn. destruct (name_eq_dec x n).
         { assert (H_n_is_fresh_2 : apply_subst s (Var n) = Var n).
-          { specialize (well_formed_subst_in_state_dom _ _ _ wfSt' n (le_refl n)).
-            intro. simpl. rewrite H0. auto. }
+          { simpl. destruct (image s n) eqn:eq; auto.
+            good_inversion wfSt'. assert (n < n).
+            { apply domLTCounter. red. eauto. }
+            omega. }
           rewrite e. rewrite H_n_is_fresh_2. simpl.
           destruct (name_eq_dec n n); try contradiction. auto. }
         { destruct (name_eq_dec x a).
@@ -772,6 +376,7 @@ Proof.
       exists s'. exists n'. split; auto. constructor; auto. } }
 Qed.
 
+
 Lemma search_completeness
       (g   : goal)
       (Hcg    : consistent_goal g)
@@ -786,7 +391,10 @@ Lemma search_completeness
 Proof.
   apply in_denotational_sem_some_lev in HDS. destruct HDS as [l HDS].
   assert (wfSt' : well_formed_state' (Leaf g empty_subst k)).
-  { constructor. red in HC. intros. apply first_nats_less; auto. }
+  { constructor.
+    { intros. good_inversion H. good_inversion H0. }
+    { intros. good_inversion H. destruct H0 as [t1 [H1 _]]. good_inversion H1. }
+    { red in HC. intros. apply first_nats_less; auto. } }
   assert (Hsubst : in_denotational_sem_subst empty_subst f).
   { red. exists f. red. intros.
     unfold subst_gt_fun_compose. rewrite apply_empty. reflexivity. }
